src/crypto/poly1305/x64/X64.Poly1305.Math_i.fsti
@@ -5,9 +5,7 @@ open X64.Machine_s   // needed for nat64
 open X64.Vale.Decls  // needed for shift_right64, logand64
 open X64.Poly1305.Spec_s // for modp
 open X64.Vale.State_i // for add_wrap
-
-let lowerUpper128 (l:nat64) (u:nat64) : nat128 =
-    0x10000000000000000 `op_Multiply` u + l
+open Bitvectors128
 
 let lowerUpper192 (l:nat128) (u:nat64) : int =
     0x100000000000000000000000000000000 `op_Multiply` u + l
@@ -121,14 +119,6 @@ val lemma_add_key : old_h0:nat64 -> old_h1:nat64 -> h_in:int -> key_s0:nat64 -> 
             (let c = old_h0 + key_s0 >= nat64_max in
              h1 == add_wrap (add_wrap old_h1 key_s1) (if c then 1 else 0)))
   (ensures lowerUpper128 h0 h1 == (h_in + key_s) % nat128_max)
-
-val lemma_lowerUpper128_and : x:nat128 -> x0:nat64 -> x1:nat64 -> y:nat128 -> y0:nat64 -> y1:nat64 -> z:nat128 -> z0:nat64 -> z1:nat64 -> Lemma
-  (requires z0 == logand64 x0 y0 /\
-            z1 == logand64 x1 y1 /\
-            x == lowerUpper128 x0 x1 /\
-            y == lowerUpper128 y0 y1 /\
-            z == lowerUpper128 z0 z1)
-  (ensures z == logand128 x y)
   
 val lemma_poly1305_heap_hash_blocks : h:int -> pad:int -> r:int -> m:mem -> i:int -> k:int{i <= k /\ (k - i) % 16 == 0 /\ (forall (j:int) . i <= j /\ j < k /\ (j - i) % 8 = 0 ==> m `Map.contains` j)} -> len:nat -> Lemma
   (requires i <= k && k <= i + len /\
