src/lib/math/Bitvectors128.fst
@@ -1,0 +1,35 @@
+module Bitvectors128
+
+open FStar.UInt
+open FStar.BV
+open FStar.Mul
+open Calc
+
+#reset-options "--smtencoding.elim_box true --z3cliopt smt.CASE_SPLIT=3 --z3rlimit 25 --z3cliopt smt.arith.nl=true --max_ifuel 0"
+
+let mod2_128 (x:int): uint_t 128 = x % 0x100000000000000000000000000000000
+
+let lemma_bv128_lowerUpper_helper1 (x1:uint_t 64) :
+  Lemma (mod2_128(x1 * 0x10000000000000000) == x1 * 0x10000000000000000) =
+  ()
+
+let lemma_bv128_lowerUpper x0 x1 =
+  calc(
+       mod2_128(mod2_128(x1 * 0x10000000000000000) + x0)
+    &= mod2_128(x1 * 0x10000000000000000 + x0) &| using 
+					 (lemma_bv128_lowerUpper_helper1 x1));
+  assume(False)
+    // lemma_bv128_lowerUpper_helper1(x1); }
+    //               { reveal_mod2_128(); }
+    //     x1 * 0x1_0000_0000_0000_0000 + x0;                     { reveal_lowerUpper128(); }
+    //     lowerUpper128(x0, x1);
+    // }
+    
+let lemma_bv128_lowerUpper_B128 (x0:uint_t 64) (x1:uint_t 64) = 
+  lemma_bv128_lowerUpper x0 x1;
+  inverse_vec_lemma #128 (bv128_64_64 (int2bv #64 x1) (int2bv #64 x0));
+  admit ()
+
+#reset-options "--smtencoding.elim_box true --z3cliopt smt.CASE_SPLIT=3 --z3rlimit 25 --z3cliopt smt.arith.nl=false --max_ifuel 0"
+let lemma_bv128_64_64_and x x0 x1 y y0 y1 z z0 z1 =
+  ()
