src/lib/math/Bitvectors128.fsti
@@ -1,0 +1,27 @@
+module Bitvectors128
+
+open FStar.UInt
+open FStar.BV
+open FStar.Mul
+
+let lowerUpper128 (l u : FStar.UInt.uint_t 64) : FStar.UInt.uint_t 128 = 
+  l + (0x10000000000000000 * u)
+let bv128_64_64 x1 x0 = bvor (bvshl (bv_uext #64 #64 x1) 64) (bv_uext #64 #64 x0)
+
+val lemma_bv128_lowerUpper : x0:uint_t 64 -> x1:uint_t 64 ->
+  Lemma(lowerUpper128 x0 x1 == bv2int (bv128_64_64 (int2bv x1) (int2bv x0)))
+
+val lemma_bv128_lowerUpper_B128 : x0:uint_t 64 -> x1:uint_t 64 ->
+  Lemma (int2bv #128 (lowerUpper128 x0 x1) == bv128_64_64 (int2bv x1) (int2bv x0))
+
+val lemma_bv128_64_64_and: x:bv_t 128 -> x0:bv_t 64 -> x1:bv_t 64 ->
+  y:bv_t 128 -> y0:bv_t 64 -> y1:bv_t 64 ->
+  z:bv_t 128 -> z0:bv_t 64 -> z1:bv_t 64 ->
+  Lemma (requires (z0 == bvand #64 x0 y0 /\
+		   z1 == bvand #64 x1 y1 /\
+		   x == bv128_64_64 x1 x0 /\
+		   y == bv128_64_64 y1 y0 /\
+		   z == bv128_64_64 z1 z0))
+	(ensures (z == bvand #128 x y))
+
+
